Initial memory parameterized by the initial stack pointer

compiler/src/main_compiler.ml
@@ -222,9 +222,9 @@ let main () =
             Format.printf "Evaluation of %s (@[<h>%a@]):@." f.fn_name
               (pp_list ",@ " pp_range) m;
             let _m, vs =
-              m |>
-              List.map (fun (ptr, sz) -> Conv.int64_of_bi ptr, Conv.z_of_bi sz) |>
-              Low_memory.Memory.coq_M.init |>
+              (** TODO: allow to configure the initial stack pointer *)
+              let live = List.map (fun (ptr, sz) -> Conv.int64_of_bi ptr, Conv.z_of_bi sz) m in
+              (match Low_memory.Memory.coq_M.init live (Conv.int64_of_bi (Bigint.of_string "1024")) with Utils0.Ok m -> m | Utils0.Error err -> raise (Evaluator.Eval_error (Coq_xH, err))) |>
               Evaluator.exec cprog (Conv.cfun_of_fun tbl f) in
             Format.printf "@[<v>%a@]@."
               (pp_list "@ " Evaluator.pp_val) vs
